now calling HSCrypto functions to avoid duplication

src/tls/KeySchedule.fst
@@ -1,86 +1,77 @@
-module KeySchedule
+module KeySchedule (*SKETCH *)
 (*the top level key schedule module, it should not expose secrets to Handshake *)
 
-type ff_all_groups =
-  | FF_2048
-  | FF_4096
-  | FF_8192
-  | FF_arbitrary of CoreCrypto.dh_params
+(* the goal is to keep ephemerals like eph_s and eph_c as currently defined 
+   in Handshake local *)
+
+open FStar.Heap
+open FStar.HyperHeap
+open FStar.Seq
+open FStar.SeqProperties // for e.g. found
+open FStar.Set  
+
+open Platform.Bytes
+open Platform.Error
+open TLSError
+open TLSConstants
+open TLSExtensions
+open TLSInfo
+open Range
+open HandshakeMessages
+open StatefulLHAE
+open HSCrypto
+
+(* For TLS12 and below only the server keeps state concretely *)
+type ks_12S =
+    | KS_12S: #region: rid -> x: rref region (KEX_S_PRIV) -> ks_12S
+    
   
-type dh_group = 
-  | FFDH of ff_all_groups
-  | ECDH of ECGroup.ec_all_curve
-
-type dh_key = 
-  | FFKey of CoreCrypto.dh_key
-  | ECKey of CoreCrypto.ec_key
-
-type dh_secret = bytes // -> abstract
-type ms = bytes // -> abstract
-
-assume val dh_keygen: g:dh_group -> Tot (x:dh_key)
-(*x contains public key share gx, 
-  in TLS 1.2 in fact used to generate y
- *)
-
-assume val dh_shared_secret1: y:dh_key -> gx:dh_key -> Tot (gxy:dh_secret)
-
-assume val dh_shared_secret2: gy:dh_key -> Tot (x:dh_key * gxy:dh_secret)
-(*x contains public key share gx*)
+(* For TLS13 both client and server keep state concretely *)    
+type ks_13C
+    | KS_13C: #region: rid -> x: rref region HSCrypto.dh_key -> ks_13C
+    ...
 
 
-
-(* TLS <= 1.2 *)
-assume val derive_keys: gxy:dh_secret -> cr:random -> sr:random -> log:bytes -> 
-	                rd:rid -> wr:rid -> i:id -> ST ((both i) * ms)
-                  //exposing ms here is problematic as it is not independent of the record keys.
-  (requires (fun h -> True))
-  (ensures (fun h0 i h1 -> True))
-
-
-val dh_init_12S: #region:rid g:dh_group -> ST (gx:dh_key)
+(* for idealization we need a top level log *)
+type state =
+  | Init
+  | Committed of ProtocolVersion * aeAlg * negotiatedExtensions
+  | Derived: a:id -> b:id -> derived a b -> state
+  
+type kdentry = CsRands * state 
+let kdlog : ref<list<kdentry>> = ref [] 
+  
+(* TLS 1.2 *)
+val dh_init_12S: #region:rid g:dh_group -> ST (state:ks_12S * gx:dh_key)
 
 let dh_init_12S r g =
   let x = dh_keygen g
   let xref = ralloc r 0 in
-  let xref := x
-  x.public //likely have to output an additional state containing the x reference
-
+  let xref := KEX_S_PRIV_DHE x
+  KS_12S r xref, x.public
   
-assume val derive_12C: #region:rid -> gx:dh_key -> ... -> ST(gy:dh_key * (both i) * ms)
+assume val derive_12C: gx:dh_key -> ... -> ST(gy:dh_key * (both i) * ms)
 
-let derive1 r gx cr sr log rd wr i = 
+let derive12C gx cr sr log rd wr i = 
   let (y, gxy) = dh_shared_secret2 gx 
   y.public, derive_keys gxy cr sr log rd wr i
 
 
-assume val derive_12S: #region:rid -> gy:dh_key -> ... -> ST ((both i) * ms)
+assume val derive_12S: state:ks_12S -> gy:dh_key -> ... -> ST ((both i) * ms)
 
-let derive_12S r gy cr sr log rd wr i =
-  let xref = lookup r //likely pass a separate state
+let derive_12S state gy cr sr log rd wr i =
+  let (KS_12S xref) = state 
   derive_keys (dh_shared_secret1 !xref) cr sr log rd wr i
 
 (* TLS 1.3 *)
-assume val derive_handshake_keys: gxy:dh_secret -> log: bytes ->
-				  rd:rid -> wr:rid -> i:id -> ST ((both i) * ms)
-  (requires (fun h -> True))
-  (ensures (fun h0 i h1 -> True))
 
-assume val derive_finished_keys: gxs:dh_secret -> gxy:dh_secret -> log: bytes -> Tot (ts:ms * cf:ms * sf:ms)
+val dh_init_13S: #region:rid g:dh_group -> ST (state:ks_13S * gs:dh_key) //s
+val dh_init_13C: #region:rid g:dh_group -> ST (state:ks_13C * gx:dh_key) //x
 
-assume val derive_traffic_keys: ts:ms -> log: bytes -> 
-				rd:rid -> wr:rid -> i:id -> ST (both i)     
-  (requires (fun h -> True))
-  (ensures (fun h0 i h1 -> True))
+assume val derive_13S_1: state:ks_13S -> gx:dh_key -> ... -> ST(gy:dh_key * (both i)) //handshake
+assume val derive_13S_2: state:ks_13S -> ... -> ST(cf:ms * sf:ms) //finished
+assume val derive_13S_3: state:ks_13S -> ... -> ST(both i) //traffic
 
-//
-val dh_init_13S: #region:rid g:dh_group -> ST (gs:dh_key) //s
-val dh_init_13C: #region:rid g:dh_group -> ST (gx:dh_key) //x
-
-assume val derive_12S_1: #region:rid -> gx:dh_key -> ... -> ST(gy:dh_key * (both i)) //handshake
-assume val derive_12S_2: #region:rid -> ... -> ST(cf:ms * sf:ms) //finished
-assume val derive_12S_3: #region:rid -> ... -> ST(both i) //traffic
-
-assume val derive_12C_1: #region:rid -> gy:dh_key -> ... -> ST(both i) //handshake
-assume val derive_12C_2: #region:rid -> gs:dh_key -> ... -> ST(cf:ms * sf:ms) //finished
-assume val derive_12C_3: #region:rid -> ... -> ST(both i) //traffic
+assume val derive_13C_1: state:ks_13C -> gy:dh_key -> ... -> ST(both i) //handshake
+assume val derive_13C_2: state:ks_13C -> gs:dh_key -> ... -> ST(cf:ms * sf:ms) //finished
+assume val derive_13C_3: state:ks_13C -> ... -> ST(both i) //traffic
